\begin{ejr}[36]
  Seas $\{ ( X_{j}, \mathcal{T}_{j} ) \}_{j \in J}$, $\{ ( X'_{j}, \mathcal{T}_{j}' ) \}_{j \in J}$ familias no vac√≠as de e.t., $( X_{j}, \mathcal{T}_{j} )$ es homeomorfo a $( X'_{j}, \mathcal{T}_{j}' )$, $\forall j \in J$. Entonces, $( \prod_{j \in J} X_{j}, \prod_{j \in J} \mathcal{T}_{j} )$ es homeomorfo a $( \prod_{j \in J} X'_{j}, \prod_{j \in J} \mathcal{T}'_{j} )$.
\end{ejr}

\begin{sol}
  Como $( X_{j}, \mathcal{T}_{j} ) \simeq( X'_{j}, \mathcal{T}_{j}' )$, entonces $\exists f_{j} : ( X_{j}, \mathcal{T}_{j} ) \to ( X'_{j}, \mathcal{T'}_{j} )$ homeomorfismo. Sea
  \[
    f : ( \prod_{j \in J} X_{j}, \prod_{j \in J} \mathcal{T}_{j} ) \to ( \prod_{j \in J} X'_{j}, \prod_{j \in J} \mathcal{T'}_{j} )
  \]
  \[ 
    f = \prod_{j \in J} f_{j} = f_{1} \times f_{2} \times \cdots 
  \] 
  donde
  \[ 
    (x_{1}, x_{2}, \cdots) \mapsto (f_{1}(x_{1}), f_{2}(x_{2}), \cdots)
  \] 
  Entonces, $f_{j}$ continua $\forall j \in J \Rightarrow f$ continua y $f_{j}^{-1}$ continua $\forall j \in J \Rightarrow f^{-1}$ continua, ya que
  \[ 
    \prod_{j \in J}(f_{j}^{-1}) = (\prod_{j \in J} f_{j}) ^{-1} 
  \] 
\end{sol}
